
# 导数

$$
\begin{matrix}
(C)' = 0; & (x^{a})' = a x^{a-1} \\
(a^{x})' = \ln a a^{x}; & (e^{x})' = e^{x} \\
(\log _{a}x)' = \frac{1}{\ln a x} & (\ln|x|)' = \frac{1}{x} \\
(\sin x)' = \cos x & (\cos x)' = -\sin x \\
(\tan x)' = \sec ^{2}x  & (\cot x)' = -\csc ^{2}x \\
(\sec x)' = \sec x \tan x & (\csc x) = -\csc x\cot x \\
(\arcsin x)' = \frac{1}{\sqrt{ 1-x^{2} }} & (\arccos x)' = -\frac{1}{\sqrt{ 1-x^{2} }} \\
(\arctan x)' = \frac{1}{1+x^{2}} & (arccot x)' = -\frac{1}{1+x^{2}}
\end{matrix}
$$

# 高阶导数

$$
\begin{matrix}
(x^{n})^{(n)} = n!  & (e^{x} )^{(n)} = e^{x} & (a^{n})^{(n)} = a^{x} \ln ^{n}a \\
(\sin x)^{(n)} = \sin\left( x + \frac{n\pi}{2} \right) & (\cos x)^{(n)} = \cos\left( x+\frac{n\pi}{2} \right)  & (\ln x)^{(n)} = (-1)^{n-1} \frac{(n-1)!}{x^{n}} \\
\left( \frac{1}{ax+b} \right)^{(n)} = (-1)^{n} \frac{a^{n}\cdot n!}{(ax+b)^{n+1}} & (\sin kx)^{(n)} = k^{n}\sin\left( kx + \frac{n\pi}{2} \right)  & (\cos kx)^{(n)} = k^{n}\cos\left( kx+ \frac{n\pi}{2} \right)
\end{matrix}
$$
# 积分

$$
\begin{matrix}
\int 0 dx = C  & \int 1 dx = x+ C \\
\int x^{a} dx = \frac{x^{a+1}}{a+1} +C & \int \frac{1}{x}dx = \ln|x| + C \\
\int a^{x} dx = \frac{a^{x}}{\ln a}+C &  \int e^{x} dx = e^{x} + C  \\
\int \sin x dx = - \cos x + C  & \int \cos x dx = \sin x +C \\
\int \tan x dx = - \ln |\cos x| dx + C  & \int \cot x dx = \ln|\sin x| +C \\
\int \sec x dx = \ln|\sec x + \tan x| + C  &  \int \csc dx = \ln|\csc x - \cot x|+C \\
\int \sec ^{2}xdx = \tan x +x & \int \csc ^{2}xdx = - \cot x + C \\
\int \frac{1}{a^{2}+x^{2}} dx = \frac{1}{a} \arctan \frac{x}{a} + C & \int \frac{1}{a^{2}-x^{2}} dx = \int \frac{1}{(a+x)(a-x)}dx = \frac{1}{2a} \left[ \int \frac{1}{a+x} dx - \int \frac{1}{a-x} dx \right]  \\
\int \frac{1}{\sqrt{ a^{2} -x^{2} }} dx = \arcsin x + C  &  \int \frac{1}{\sqrt{ x^{2}\pm a^{2} }} dx = \ln|x+\sqrt{ x^{2}\pm a^{2} }| +C
\end{matrix}
$$




